a) $(a,b)\in ]0,1]^2 \Rightarrow ab \in ]0,1] \Rightarrow ab-1\leq 0$. De même $bc-1\leq 0$ et $ac-1\leq 0$, donc on a le produit de trois nombres négatifs: $(ab-1)(bc-1)(ac-1)\leq 0$. \\
b) Développons et divisons par $abc > 0$:
\begin{eqnarray}
  (ab-1)(bc-1)(ac-1)\leq 0 & \Leftrightarrow & a^2b^2c^2-a^2bc-ab^2c-abc^2 + ab + bc+ac-1 \leq 0 \nonumber \\
   & \Leftrightarrow & a^2b^2c^2+ ab + bc+ac \leq 1 + a^2bc+ ab^2c + abc^2 \nonumber \\
   & \Leftrightarrow & abc + \frac{1}{c} + \frac{1}{b} + \frac{1}{a}  \leq + \frac{1}{abc} + a+b+c \nonumber
\end{eqnarray}
