$\frac{\pi}{12} = \frac{4\pi}{12} - \frac{3\pi}{12}=\frac{\pi}{3}-\frac{\pi}{4}$ donc:
\begin{eqnarray}
  \cos\left(\frac{\pi}{12}\right) &=& \cos\left(\frac{\pi}{3}-\frac{\pi}{4}\right) \nonumber \\
    &=& \cos\left(\frac{\pi}{3}\right)\cos\left(\frac{\pi}{4}\right)+\sin\left(\frac{\pi}{3}\right)\sin\left(\frac{\pi}{4}\right)  \nonumber \\
   &=& \frac{1}{2}\frac{\sqrt{2}}{2} + \frac{\sqrt{3}}{2}\frac{\sqrt{2}}{2} \nonumber \\
                      &=&  \frac{\sqrt{2}\left(1+\sqrt{3}\right)}{4} \nonumber
\end{eqnarray}
