Comme tout est strictement positif, on a:
\begin{eqnarray*}
  \frac{a}{a'} > \frac{b}{b'} &\Rightarrow& ab' > a'b \\
  &\Rightarrow& nab' > na'b \\
  &\Rightarrow& maa'+ nab' > maa'+na'b \\
  &\Rightarrow& a(ma'+ nb') > a'(ma+nb) \\
  &\Rightarrow& \frac{ma'+ nb'}{ma+nb} < \frac{a}{a'}
\end{eqnarray*}
De la même manière:
\begin{eqnarray*}
  \frac{a}{a'} > \frac{b}{b'} &\Rightarrow& ab' > a'b \\
  &\Rightarrow& mab' > ma'b \\
  &\Rightarrow& nbb'+ mab' > nbb'+ma'b \\
  &\Rightarrow& b'(ma + nb') > b(ma'+nb') \\
  &\Rightarrow&  \frac{b}{b'} < \frac{ma'+ nb'}{ma+nb}
\end{eqnarray*}
Finalement,
\[
\frac{b}{b'} < \frac{ma'+ nb'}{ma+nb} < \frac{a}{a'}
\]
